Strata/DL/Lambda/LTyUnify.lean
@@ -103,28 +103,20 @@ theorem SubstWF.single_subst (id : TyIdentifier) (h : ¬id ∈ ty.freeVars) :
 
 theorem Subst.mem_freeVars_of_mem_freeVars_remove (S : Subst) (id : TyIdentifier)
   (h : xty ∈ Subst.freeVars (Maps.remove S id)) :
-  xty ∈ Subst.freeVars s := by
-  induction S
-  case nil => simp_all [Maps.remove]
-  case cons head tail tail_ih =>
-    sorry
-    stop
-    by_cases h_id_head : head.fst = id
-    case pos =>
-      simp_all [Map.remove]
-    case neg =>
-      simp_all [Map.remove]
-      cases h <;> try simp_all
+  xty ∈ Subst.freeVars S := by
+  simp_all [Subst.freeVars]
+  obtain ⟨aty, h1, h2⟩ := h
+  apply Exists.intro aty; simp_all
+  simp [@Maps.mem_values_of_mem_keys_remove _ _ _ _ S id aty h1]
 
 theorem SubstWF_of_remove (id : TyIdentifier) (h : SubstWF S) :
   SubstWF (Maps.remove S id) := by
-  -- simp_all [SubstWF]
-  -- intro xty h_xty_in_keys h_xty_in_fvs
-  -- have h_xty_in_s_keys := @Map.mem_keys_of_mem_keys_remove _ _ _ s id xty h_xty_in_keys
-  -- have h_xty_not_in_fvs := @h xty h_xty_in_s_keys
-  -- have := @Subst.mem_freeVars_of_mem_freeVars_remove xty s id h_xty_in_fvs
-  -- contradiction
-  sorry
+  simp_all [SubstWF]
+  intro xty h_xty_in_keys h_xty_in_fvs
+  have h_xty_in_s_keys := @Maps.mem_keys_of_mem_keys_remove _ _ _ _ S id xty h_xty_in_keys
+  have h_xty_not_in_fvs := @h xty h_xty_in_s_keys
+  have := @Subst.mem_freeVars_of_mem_freeVars_remove xty S id h_xty_in_fvs
+  contradiction
 
 /--
 A type substitution, along with a proof that it is well-formed.
@@ -1112,7 +1104,7 @@ def Constraints.unify (constraints : Constraints) (S : SubstInfo) :
 /-- info: ok: [(a, int) (b, (arrow c d))] -/
 #guard_msgs in
 open LTy.Syntax in
-#eval!  do let S ← Constraints.unify [(mty[%a → %b], mty[int → (%c → %d)])] SubstInfo.empty
+#eval  do let S ← Constraints.unify [(mty[%a → %b], mty[int → (%c → %d)])] SubstInfo.empty
            return (format S.subst)
 
 ---------------------------------------------------------------------
